fix automation

refinedVST/typing/automation.v
@@ -242,6 +242,13 @@ Ltac liRJudgement :=
       (* notypeclasses refine (tac_fast_apply (type_addr_of_place _ _ _ _) _); [solve [refine _] |] *)
   end.
 
+(* deal with objective modalities. This is ad-hoc for now *)
+Ltac liObj :=
+  match goal with
+  | |- envs_entails _ (<obj> _) =>
+    iModIntro
+  end.
+
 (* This does everything *)
 Ltac liRStep :=
  liEnsureInvariant;
@@ -252,6 +259,7 @@ Ltac liRStep :=
  (* | liRIntroduceTypedStmt *)
  | liRExpr
  | liRJudgement
+ | liObj
  | liStep
 ]; liSimpl.
 
@@ -366,12 +374,8 @@ Section automation_tests.
   Proof.
     iIntros.
     repeat liRStep.
-    
-    Admitted.
-    (* do 30 liRStep.
     liShow; try done.
- (** TODO make use of Objective environment *)
-  Qed. *)
+  Qed.
 
   Goal forall Espec Delta (_x:ident) b o (l:address) ty ,
   TCDone (ty_has_op_type ty tint MCNone) ->
@@ -417,16 +421,40 @@ End automation_tests.
 
 From VST.typing Require Import automation_test.
 
+Global Instance related_to_val_embed `{!typeG Σ} {cs : compspecs} A v ty : RelatedTo (λ x : A, (⎡v ◁ᵥ ty x⎤:(monPredI environ_index (ouPredI (iResUR Σ)))))%I | 100
+:= {| rt_fic := FindVal v |}.
+Global Instance related_to_val_embed2 `{!typeG Σ} {cs : compspecs} A v ty : RelatedTo (λ x : A, (⎡v ◁ᵥ ty⎤:(monPredI environ_index (ouPredI (iResUR Σ)))))%I | 100
+:= {| rt_fic := FindVal v |}.
+
+Arguments find_in_context : simpl never.
+Arguments subsume : simpl never.
+Arguments FindVal  : simpl never.
+
+Lemma simple_subsume_val_to_subsume_embed `{!typeG Σ} `{compspecs} (A:Type) (v : val) (ty1 : type) (ty2 : A → type) (P:A->mpred)
+  `{!∀ (x:A), SimpleSubsumeVal ty1 (ty2 x) (P x)} (T: A-> assert) :
+   (∃ x, (@embed mpred assert _ $ P x) ∗ T x) ⊢@{assert} subsume (⎡v ◁ᵥ ty1⎤) (λ x : A, ⎡v ◁ᵥ ty2 x⎤) T.
+Proof.
+  iIntros "H".
+  iDestruct "H" as (x) "[HP HT]".
+  unfold subsume. iIntros. iExists x. iFrame.
+  iStopProof; go_lowerx.
+  iIntros "[HP Hv]".
+  iApply (@simple_subsume_val with "HP Hv").
+Qed.
+
+Definition simple_subsume_val_to_subsume_embed_inst `{!typeG Σ} `{compspecs} := [instance simple_subsume_val_to_subsume_embed].
+Global Existing Instance simple_subsume_val_to_subsume_embed_inst.
+
   Module f_test1.
     Context `{!typeG Σ} {cs : compspecs} `{!externalGS OK_ty Σ}.
   
     Opaque local locald_denote.
 
     Definition spec_f_ret_expr :=
-      fn(∀ () : (); <affine> True) → ∃ z : Z, int tint ; <absorb> ⌜z=42⌝.
+      fn(∀ () : (); emp) → ∃ z : Z, (z @ ( int tint )); ⌜z = 3⌝.
     Instance CompSpecs : compspecs. make_compspecs prog. Defined.
     Definition Vprog : varspecs. mk_varspecs prog. Defined.
-    Definition Delta := (func_tycontext f_f_ret_expr Vprog [] []).
+    Local Definition Delta := (func_tycontext f_f_ret_expr Vprog [] []).
 
     Goal forall Espec, ⊢ typed_function(A := ConstType _) Espec Delta f_f_ret_expr spec_f_ret_expr.
     Proof.
@@ -439,46 +467,111 @@ From VST.typing Require Import automation_test.
       let lsa := fresh "lsa" in
       let lsb := fresh "lsb" in
       let rho := fresh "rho" in
-      iIntros "!#" (lsa lsb rho). inv_vec lsb. inv_vec lsa.
+      iIntros "!#" (lsa lsb). inv_vec lsb. inv_vec lsa.
     
-      simpl. 
-      (* TODO go_higher here? *)
-      (* simpl. *)
+      iPureIntro.
+      iIntros "(?&?&?&?)".
+      simpl.
+      
+      liRStep.
+      liRStep.
+      
+      
+      liRStep.
+      liRStep.
+      liRStep.
+      liRStep.
+      liRStep.
+      liRStep.
+      liRStep.
+      liRStep.
+      liRStep.
+      
+      liRStep.
+      liRStep.
+      
+      unfold LET_GOAL, LET_ID.
+      liRStep.
 
-      rewrite -?(@monPred_at_emp environ_index mpred rho)
-              -?(@monPred_at_pure environ_index mpred rho) 
-              -?(monPred_at_affinely) 
-              -?monPred_at_sep 
-              -?monPred_wand_force.
+      unfold LET_GOAL, LET_ID.
+      liRStep.
+      liRStep.
+      liRStep.
+      liRStep.
 
-      Lemma go_higher : forall (P: assert) rho,
-        @bi_emp_valid (assert) P -> ⊢ monPred_at P rho.
-      Proof. 
-        intros ???.
-        destruct H as [H].
-        by iApply (H rho).
+      (* liRStep. *)
+
+Ltac push_in_embed_setoid :=
+    (* try setoid_rewrite embed_wand;
+    try setoid_rewrite embed_wand_iff;
+    try setoid_rewrite embed_forall;
+    try setoid_rewrite embed_exist;
+    try setoid_rewrite embed_and;
+    try setoid_rewrite embed_or;
+    try setoid_rewrite embed_impl;
+    try setoid_rewrite embed_iff;
+    try setoid_rewrite embed_sep; *)
+    try setoid_rewrite embed_pure;
+    try setoid_rewrite embed_emp;
+    try setoid_rewrite embed_affinely;
+    (* try setoid_rewrite embed_persistently;
+    try setoid_rewrite embed_absorbingly;
+    try setoid_rewrite embed_embed;
+    try setoid_rewrite embed_bupd;
+    try setoid_rewrite embed_fupd;
+    try setoid_rewrite embed_intuitionistically;
+    try setoid_rewrite embed_except_0;
+    try setoid_rewrite embed_later;
+    try setoid_rewrite embed_laterN;
+    try setoid_rewrite embed_plainly;
+    try setoid_rewrite embed_plainly_if;
+    try setoid_rewrite embed_affinely_if;
+    try setoid_rewrite embed_persistently_if;
+    try setoid_rewrite embed_absorbingly_if;
+    try setoid_rewrite embed_intuitionistically_if;
+    try setoid_rewrite embed_internal_eq;
+    (* not sure how to deal with other forms in `bi_embed $ monPred_at ...`, add them when in need *)
+    try setoid_rewrite monPred_at_sep;
+    try setoid_rewrite monPred_at_affinely *)
+    idtac
+    .
+
+
+      Ltac push_in_embed_for_head ::=
+      idtac "ahhh";
+      let push_in_embed_inside_term H :=
+        match H with | context [@embed ?p1 ?p2 _ ?H] => push_in_embed (@embed p1 p2 _ H) end in
+      lazymatch goal with
+      | |- envs_entails ?Δ ?P =>
+        lazymatch P with
+        | embed ?H => push_in_embed_inside_term H
+        | bi_wand ?H _ => push_in_embed_inside_term H
+        | bi_sep ?H _ => push_in_embed_inside_term H
+        | bi_exist ?H => idtac H; progress push_in_embed_setoid
+        (* | ?un_op ?H => idtac "unop" un_op; push_in_embed H
+        | ?bin_op ?H _ => idtac "binop" bin_op; push_in_embed H *)
+        end end.
+         (* FIXME rewrite is too aggresive *)
+      
+      liRStep.
+      liRStep.
+      liRStep.
+      liRStep.
+      liRStep.
+      liRStep.
+      
+      (* TODO liSep for (pure _ ∗ _)? *)
+      iSplit. - iPureIntro. reflexivity. 
+      - liRStep.
       Qed.
-
-      iApply go_higher.
-      iStartProof.
-
-      liRStep.
-      liRStep.
-      liRStep.
-      liRStep.
-      liRStep.
-      liRStep.
-      liRStep.
-      repeat liRStep.
-      (* do Sreturn here *)
-    Admitted.
   End f_test1.
 
   Module f_test2.
     Context `{!typeG Σ} {cs : compspecs} `{!externalGS OK_ty Σ}.
 
     Definition spec_f_temps :=
-      fn(∀ () : (); emp) → ∃ z : Z, int tint ; <absorb> ⌜z=42⌝.
+      fn(∀ () : (); emp) → ∃ z : Z, (z @ (int tint)) ; ⌜z=42⌝.
+
     Local Instance CompSpecs : compspecs. make_compspecs prog. Defined.
     Local Definition Vprog : varspecs. mk_varspecs prog. Defined.
     (* Local Definition Delta := (func_tycontext f_f_temps Vprog [] []). *)
@@ -494,8 +587,7 @@ From VST.typing Require Import automation_test.
       { iPureIntro; simpl. repeat constructor. }
       let lsa := fresh "lsa" in
       let lsb := fresh "lsb" in
-      let rho := fresh "rho" in
-      iIntros "!#" (lsa lsb rho). inv_vec lsb. inv_vec lsa.
+      iIntros "!#" (lsa lsb). inv_vec lsb. inv_vec lsa.
 
       simpl.
       rewrite -?(@monPred_at_emp environ_index mpred rho)
@@ -511,14 +603,9 @@ From VST.typing Require Import automation_test.
       destruct H as [H].
       by iApply (H rho).
     Qed.
-
-    iApply go_higher.
-    iStartProof.
-
+    iPureIntro.
+    iIntros "(?&?&?&?)".
     repeat liRStep.
-    iIntros.
-    iModIntro.
-    repeat liRStep.
-    unfold IPM_JANNO.
+  Admitted.
 
-End automation_tests.
+End f_test2.
